cryptis/primitives/pre_term.v
@@ -110,12 +110,35 @@ Definition leq_term : val := rec: "loop" "t1" "t2" :=
     else #false
   else #false)%V.
 
-Definition texp : val := λ: "t1" "t2",
-  if: Fst "t1" = #TExp_tag then
-    let: "base" := Fst (Snd "t1") in
-    let: "exp"  := Snd (Snd "t1") in
-    (#TExp_tag, ("base", insert_sorted leq_term "t2" "exp"))
-  else (#TExp_tag, ("t1", ["t2"])).
+(* TODO: Better names / separate file *)
+Definition hl_base : val := λ: "pt",
+    if: Fst "pt" = #TExp_tag then
+        Fst (Snd "pt")
+    else "pt".
+
+Definition hl_exps : val := λ: "t",
+    if: Fst "t" = #TExp_tag then
+        Snd (Snd "t")
+    else NILV.
+
+Definition hl_inv : val := λ: "pt",
+    if: Fst "pt" = #TOp1_tag then
+        if: Fst (Fst (Snd "pt")) = #TInv_tag then Snd (Snd "pt")
+        else (#TOp1_tag, (#TInv_tag, #(), "pt"))
+    else (#TOp1_tag, (#TInv_tag, #(), "pt")).
+
+Definition hl_insert_exp : val := λ: "pt" "pts",
+    if: mem_list eq_term (hl_inv "pt") "pts" then
+        rem_list eq_term (hl_inv "pt") "pts"
+    else "pt" :: "pts".
+
+Definition hl_cancel_exps : val := λ: "exps", foldr_list hl_insert_exp [] "exps".
+
+Definition hl_exp : val := λ: "pt" "pts",
+    let: "normed" := insertion_sort leq_term (
+        hl_cancel_exps (append_lists (hl_exps "pt") "pts")) in
+    if: "normed" = [] then hl_base "pt"
+    else (#TExp_tag, (hl_base "pt", "normed")).
 
 Section Proofs.
 
@@ -286,6 +309,111 @@ iIntros "post"; wp_rec; wp_pures; try by iApply "post".
     move=> ????; iIntros "_ post".
     by rewrite /=; iApply IHts1 => //; iApply "post".
   + by iIntros "_".
+Qed.
+
+Lemma twp_hl_base E (pt : PreTerm.pre_term) :
+    [[{ True }]] hl_base (repr pt) @ E [[{ RET repr (PreTerm.base pt); True }]].
+Proof.
+    case: pt => * /=; iIntros "_ HΦ"; wp_lam; wp_pures; by iApply "HΦ".
+Qed.
+
+(* TODO: Is this already proved somewhere else? *)
+Lemma repr_pre_term_list (pts : seq PreTerm.pre_term) :
+    repr_list (ListDef.map val_of_pre_term pts) = repr_list pts.
+Proof.
+    rewrite !repr_list_unseal.
+    assert (
+        list.foldr (λ (x : heap_lang.val) v, InjRV (repr x, v))
+            (InjLV #()) (val_of_pre_term <$> pts) =
+        list.foldr (λ (x : PreTerm.pre_term) v,
+            InjRV (repr (val_of_pre_term x), v)) (InjLV #()) pts
+    ) by by rewrite foldr_fmap.
+    simpl in H. rewrite -H. reflexivity.
+Qed.
+
+Lemma twp_hl_exps E (pt : PreTerm.pre_term) :
+    [[{ True }]] hl_exps (repr pt) @ E [[{ RET repr (PreTerm.exps pt); True }]].
+Proof.
+    case: pt => * /=; iIntros "_ HΦ"; wp_lam; wp_pures;
+        rewrite ?repr_pre_term_list repr_list_unseal; by iApply "HΦ".
+Qed.
+
+Lemma twp_hl_inv E (pt : PreTerm.pre_term) :
+    [[{ True }]] hl_inv (repr pt) @ E [[{ RET repr (PreTerm.inv pt); True }]].
+Proof.
+    case: pt => [*|t *|*|*] /=; iIntros "_ HΦ";
+        try case: t => * /=; wp_lam; wp_pures; by iApply "HΦ".
+Qed.
+
+(* TODO: Is this already proved somewhere else? *)
+Lemma eq_equiv x y : bool_decide (x = y) = (x == y).
+Proof. Admitted.
+
+Lemma twp_hl_insert_exp E (pt : PreTerm.pre_term) (pts : seq PreTerm.pre_term) :
+    [[{ True }]]
+        hl_insert_exp (repr pt) (repr pts) @ E
+    [[{ RET repr (PreTerm.insert_exp pt pts); True }]].
+Proof.
+    iIntros "%Φ _ HΦ".
+    rewrite /PreTerm.insert_exp.
+    wp_lam; wp_pures.
+    wp_apply twp_hl_inv => //; iIntros "_".
+    wp_apply twp_mem_list => //.
+        iIntros "%x %y %Ψ _ HΨ". wp_apply twp_eq_pre_term.
+        rewrite eq_equiv. by iApply "HΨ".
+        iIntros "_".
+    case: (PreTerm.inv pt \in pts); wp_pures.
+        - wp_apply twp_hl_inv => //; iIntros "_".
+          wp_apply twp_rem_list => //.
+          iIntros "%x %y %Ψ _ HΨ". wp_apply twp_eq_pre_term.
+          rewrite eq_equiv. by iApply "HΨ".
+        - wp_apply twp_cons. by iApply "HΦ".
+Qed.
+
+Lemma twp_hl_cancel_exps E (pts : seq PreTerm.pre_term):
+    [[{ True }]]
+        hl_cancel_exps (repr pts) @ E
+    [[{ RET (repr (PreTerm.cancel_exps pts)); True }]].
+Proof.
+    iIntros "%Φ _ HΦ"; wp_lam; wp_pures.
+    wp_apply twp_nil.
+    wp_apply twp_foldr_list => //.
+    iIntros "%a %b %Ψ _ HΨ".
+    wp_apply twp_hl_insert_exp => //.
+Qed.
+
+Lemma twp_hl_exp E (pt : PreTerm.pre_term) (pts : seq PreTerm.pre_term) :
+    [[{ True }]]
+        hl_exp (repr pt) (repr pts) @ E
+    [[{ RET repr (PreTerm.exp pt pts); True }]].
+Proof.
+    iIntros "%Φ _ HΦ"; wp_lam.
+    wp_pures.
+    wp_apply twp_hl_exps; first done; iIntros "_".
+    wp_apply twp_append_lists; first done; iIntros "_".
+    wp_apply twp_hl_cancel_exps; first done; iIntros "_".
+    simpl; wp_apply twp_insertion_sort.
+        iIntros "%x %y %Ψ _ HΨ". iApply twp_leq_pre_term. by iApply "HΨ".
+        done. iIntros "_".
+    wp_pures.
+    rewrite /PreTerm.exp.
+    set normed := (sort <=%O (PreTerm.cancel_exps (PreTerm.exps pt ++ pts)%list)).
+    destruct (decide (size normed = 0)) as [H | H].
+        rewrite H. iSimpl in "HΦ".
+        rewrite (size0nil H); rewrite repr_list_unseal; simpl.
+        wp_pures.
+        by wp_apply twp_hl_base.
+    assert ((@eq_op
+        ssrnat.Datatypes_nat__canonical__eqtype_Equality (* Why *)
+        (size normed) 0) = false) as -> by by destruct normed.
+    assert (bool_decide (repr_list normed = NONEV) = false) as Hhl
+        by (destruct normed; by rewrite repr_list_unseal);
+        rewrite Hhl; clear Hhl. (* This works, but `as ->` doesn't *)
+    wp_pures.
+    wp_apply twp_hl_base => //; iIntros "_".
+    wp_pures.
+    iSimpl in "HΦ". rewrite repr_pre_term_list.
+    by iApply "HΦ".
 Qed.
 
 End Proofs.
